verified/sec_prop.s.dfy
@@ -1,12 +1,6 @@
 include "smcapi.s.dfy"
-//include "pagedb.i.dfy"
 include "pagedb.s.dfy"
-// I need this until we figure out how to extract just the trusted parts
-// include "ptables.i.dfy"
 
-/* 
- * If I recall correctly these exist / existed elsewhere... dig later
- */
 predicate valDispPage(d: PageDb, n: PageNr)
     requires validPageDb(d)
 {
@@ -47,20 +41,6 @@ predicate usr_regs_equiv(s1:state, s2:state)
     s1.regs[LR(User)] == s2.regs[LR(User)]
 }
 
-// TODO somehow this broke... put it back...
-// Like WritablePagesInTable but includes pages without the write bit set
-/*
-function PagesInTable(pt:AbsPTable): set<addr>
-    requires WellformedAbsPTable(pt)
-    ensures forall m:addr :: m in PagesInTable(pt) ==> PageAligned(m)
-{
-    (set i, j | 0 <= i < |pt| && pt[i].Just? && 0 <= j < |pt[i].v|
-        && pt[i].v[j].Just?
-        :: (assert WellformedAbsPTE(pt[i].v[j]);
-          pt[i].v[j].v.phys + PhysBase()))
-}
-*/
-
 //-----------------------------------------------------------------------------
 //  Confidentiality, Malicious Enclave
 //-----------------------------------------------------------------------------
@@ -90,15 +70,7 @@ predicate {:opaque} enc_conf_eqpdb(d1:PageDb, d2: PageDb, atkr:PageNr)
         d1[n].entry == d2[n].entry)))
 }
 
-// This relation is used to describe two states from which attacker entry 
-// begins. It isused to set sources of nondeterminism equal so 
-// that we can reason about what the attacker observes during execution without 
-// needing to prove that this nondeterministic system is deterministic.
-
-// The entry spec can pass around the value bad_enclave to each of the 
-// existentially reached states so that we can assume sources of nondeterminism 
-// for each state reached after the executions beginning from s1 and s2
-
+// TODO: this is no longer a function of anything other than the states...
 predicate enc_conf_eq_entry(s1:state, s2:state, d1:PageDb, d2:PageDb, 
     atkr:PageNr)
     requires ValidState(s1) && ValidState(s2)
@@ -112,14 +84,31 @@ predicate enc_conf_eq_entry(s1:state, s2:state, d1:PageDb, d2:PageDb,
 // Confidentiality, Malicious OS
 //-----------------------------------------------------------------------------
 
-predicate os_conf_eq(s1: state, s2: state)
+predicate {:opaque} os_conf_eqpdb(d1:PageDb, d2:PageDb)
+    requires validPageDb(d1) && validPageDb(d2)
+{
+    (forall n: PageNr ::
+        d1[n].PageDbEntryTyped? <==> d2[n].PageDbEntryTyped?) &&
+    (forall n: PageNr | d1[n].PageDbEntryTyped? &&
+        (d1[n].entry.Addrspace? || d1[n].entry.L1PTable? || 
+            d1[n].entry.L2PTable?) ::
+                d1[n].entry == d2[n].entry) &&
+    (forall n : PageNr | d1[n].PageDbEntryTyped? && d1[n].entry.Dispatcher? ::
+        d2[n].entry.Dispatcher? && d1[n].entry.entered == d2[n].entry.entered) &&
+    (forall n : PageNr | d1[n].PageDbEntryTyped? && d1[n].entry.DataPage? ::
+        d2[n].entry.DataPage?)
+}
+
+predicate os_conf_eq(s1: state, d1: PageDb, s2: state, d2: PageDb)
     requires ValidState(s1) && ValidState(s2)
+    requires validPageDb(d1) && validPageDb(d2)
 {
     reveal_ValidMemState();
     s1.conf.nondet == s2.conf.nondet &&
     os_regs_equiv(s1, s2) &&
-    os_ctrl_eq(s1, s2) // &&
-    // InsecureMemInvariant(s1, s2)
+    os_ctrl_eq(s1, s2) &&
+    InsecureMemInvariant(s1, s2) &&
+    os_conf_eqpdb(d1, d2)
 }
 
 predicate os_ctrl_eq(s1: state, s2: state)
@@ -192,26 +181,3 @@ predicate enc_integ_eqpdb(d1:PageDb, d2: PageDb, atkr:PageNr)
             d1[n].addrspace == d2[n].addrspace &&
             d1[n].entry == d2[n].entry)
 }
-
-/*
-predicate enc_integ_eq(s1:state, s2:state, d1:PageDb, d2:PageDb, 
-    atkr:PageNr)
-    requires SaneState(s1) && SaneState(s2)
-    requires validPageDb(d1) && validPageDb(d2)
-    requires pageDbCorresponds(s1.m, d1) && pageDbCorresponds(s2.m, d2)
-{
-    s1.public == s2.public &&
-    valAddrPage(d1, atkr) && valAddrPage(d2, atkr) &&
-    (var l1p := d1[atkr].entry.l1ptnr; // same in both d1, d2 because of eqdb
-    nonStoppedL1(d1, l1p) <==> nonStoppedL1(d2, l1p) &&
-    nonStoppedL1(d1, l1p) ==> (
-        var atkr_pgs := WritablePagesInTable(mkAbsPTable(d1, l1p));
-        // The set of pages the attacker can modify is the same
-        (WritablePagesInTable(mkAbsPTable(d1, l1p)) == 
-            WritablePagesInTable(mkAbsPTable(d2, l1p))) &&
-        // The contents of pages the attacker cannot modify is the same
-        (forall a | a in TheValidAddresses() && a !in atkr_pgs::
-            s1.m.addresses[a] == s2.m.addresses[a])
-    ))
-}
-*/
