verified/sec_prop_util.i.dfy
@@ -3,6 +3,10 @@ include "pagedb.s.dfy"
 include "entry.s.dfy"
 include "sec_prop_util.i.dfy"
 
+//-----------------------------------------------------------------------------
+// Enclave Confidentiality
+//-----------------------------------------------------------------------------
+
 predicate ni_reqs(s1: state, d1: PageDb, s1': state, d1': PageDb,
                   s2: state, d2: PageDb, s2': state, d2': PageDb,
                   atkr: PageNr)
@@ -65,4 +69,18 @@ predicate entering_atkr(d1: PageDb, d2: PageDb, disp: word, atkr: PageNr, is_res
     nonStoppedDispatcher(d1, disp) && nonStoppedDispatcher(d2, disp) &&
     smc_enter_err(d1, disp, is_resume) == KOM_ERR_SUCCESS &&
     smc_enter_err(d2, disp, is_resume) == KOM_ERR_SUCCESS
+}
+
+//-----------------------------------------------------------------------------
+// OS Confidentiality
+//-----------------------------------------------------------------------------
+
+predicate os_ni_reqs(s1: state, d1: PageDb, s1': state, d1': PageDb,
+                     s2: state, d2: PageDb, s2': state, d2': PageDb)
+{
+    ValidState(s1) && validPageDb(d1) && ValidState(s1') && validPageDb(d1') &&
+    ValidState(s2) && validPageDb(d2) && ValidState(s2') && validPageDb(d2') &&
+    SaneConstants() //&&
+    // pageDbCorresponds(s1.m, d1) && pageDbCorresponds(s1'.m, d1') &&
+    // pageDbCorresponds(s2.m, d2) && pageDbCorresponds(s2'.m, d2')
 }
